---
layout: post
title:  "Math behind Euclid's theorem"
date:   2020-04-26 00:00:00 -0400
tags: advanced application math
excerpt: Wondered why Euclid's GCD theorem works?
---

We were taught in our programming classes that, to calculate gcd of two integers **efficiently** use the Euclid's algorithm.

## Magic

The Euclid algorithm is programmed as follows:

```python
def gcd(a: int, b: int) -> int:
    # hatch case
    if a == 0:
        return b
    else:
        return gcd(b % a, a)

assert gcd(15, 6) == 3
```

Take a step back and think for a minute. Why does it work?

## How did you do that?

I will explain this with the magic as the starting point to end up stating the Euclid's theorem. Reverse Engineering!

### Rewriting the code

```python
def gcd(a: int, b: int) -> int:
    while a != 0:
        # to keep it descriptive
        tmp = b % a
        b = a
        a = tmp
    return b

assert gcd(15, 6) == 3
```

Now carefully understand the following,

![Formula](/assets/img/math-euclid/formula.png)

`%` is not a basic arithmetic operator in mathematics. Consider the following implementation of `%` function:

```python
'''
b % a
'''
def mod(b: int ,a: int) -> int:
    tmp = b
    while tmp >= a:
        tmp = tmp - a
    return tmp

assert mod(15, 6) == 15 % 6
```

Now, Let's replace the mod function with its implementation in the former code snippet.

```python
def gcd(a: int, b: int) -> int:
    while a != 0:
        # replacement BEGIN
        tmp = b
        while tmp >= a:
            tmp = tmp - a
        # replacement END
        b = a
        a = tmp
    return b

assert gcd(15, 6) == 3
```

## Wrap-up

To understand better, let us optimize the code to make analysis easier. Observe that `b` takes the value of a after `n` `a`'s are removed from it, and `a` is given the processed `b` value. Consider the second iteration. If the values were swapped, the code runs as expected. But, if they were not swapped, then we need to make an edition such that `tmp` takes `a`, the condition becomes `tmp >= b`, and the loop-code is `tmp = tmp-b`. Let's make these changes to the code and merge the loops.

```python
def gcd(a: int, b: int) -> int:
    while a != 0 and b != 0:
        if a >= b:
            a = a - b
        else:
            b = b - a
    # loop breaks when either one is 0
    return a if b == 0 else b

assert gcd(15, 6) == 3
```

Take a moment to understand and verify the code snippet.
Thus, we observe that `gcd(a, b) = gcd(a-b, b) = gcd(a, b-a)`.

Let, `d` be a factor of both `a` and `b`. Hence, `d|a` (d divides a) and `d|b` (d divides b).

In mathematical form, `a = dx, b = dy`, where `x`, `y` are Integers (`Z`).

```
a - b = dx - dy
=> a - b = d(x - y)
and, 
b - a = dy - dx
=> b - a = d(y - x)
```

Hence, `d|a`, `d|b`, `d|(a-b)` and `d|(b-a)`. The least positive `d` that we finally end up is the GCD of `a` and `b`.

Now traceback through this article, to understand why Euclid's GCD theorem works.